SystemF2Data: fixing prim related holes
Ignore-this: ab8363caef2929f148f17579bdea7e86

darcs-hash:20130424050043-08f32-7d2ff03b435666e766e033f5e11a9fe8ded3fc36

done/Iron/Language/SystemF2Data/Exp/Base.v
@@ -1,20 +1,6 @@
 
 Require Export Iron.Language.SystemF2Data.Type.
-
-Inductive prim : Type :=
- | PNat    : nat  -> prim 
- | PBool   : bool -> prim
-
- | PAdd    : prim
- | PIsZero : prim.
-
-
-Inductive defprim : Type :=
- | DefPrim 
-   :  list ty    (* Types of the arguments. *)
-   -> ty         (* Type  of the returned value. *)
-   -> defprim.
-
+Require Export Iron.Language.SystemF2Data.Exp.Prim.
 
 
 (* Expressions *)
