done/Iron/Language/SystemF2Data/Exp/Prim.v
@@ -1,0 +1,84 @@
+
+Require Import Iron.Language.SystemF2Data.Type.
+
+
+(* Primive operators and literals. *)
+Inductive prim : Type :=
+ (* Literal natural number. *)
+ | PNat    : nat  -> prim 
+
+ (* Literal boolean. *)
+ | PBool   : bool -> prim
+
+ (* Add two naturals. *)
+ | PAdd    : prim
+
+ (* Check whether a natural is zero. *)
+ | PIsZero : prim.
+
+
+(* Primitive operator definition.
+   We keep the types of primops separate from the main typing judgement
+   to make it easy to add new ones. *)
+Inductive defprim : Type :=
+ | DefPrim 
+   :  list ty    (* Types of the arguments. *)
+   -> ty         (* Type  of the returned value. *)
+   -> defprim.
+
+
+(* Define the types of primops. *)
+Fixpoint primDef (p : prim) : defprim := 
+ match p with
+ | PNat  _   => DefPrim nil (TCon TyConNat)
+ | PBool _   => DefPrim nil (TCon TyConBool)
+ | PAdd      => DefPrim (TCon TyConNat :: TCon TyConNat :: nil) (TCon TyConNat)
+ | PIsZero   => DefPrim (TCon TyConNat :: nil)                  (TCon TyConBool)
+ end. 
+
+
+(********************************************************************)
+(* The types of all primops are closed. *)
+Lemma prim_types_closed
+ :   forall p ts t
+ ,   primDef p = DefPrim ts t
+ ->  Forall closedT ts
+  /\ closedT t.
+Proof.
+ intro.
+ destruct p; snorm;
+  try (solve [inverts H; nope]);
+  try (solve [inverts H; eauto]).
+
+ + inverts H.
+   inverts H0. eauto.
+   inverts H.  eauto.
+   nope.
+
+ + inverts H.
+   inverts H0. eauto.
+   inverts H.
+Qed.
+Hint Resolve prim_types_closed.
+
+
+Lemma prim_types_closed_args
+ :  forall p ts t
+ ,  primDef p = DefPrim ts t
+ -> Forall closedT ts.
+Proof.
+ intros. eapply prim_types_closed in H; rip.
+Qed.
+Hint Resolve prim_types_closed_args.
+
+
+Lemma prim_types_closed_result
+ :  forall p ts t
+ ,  primDef p = DefPrim ts t
+ -> closedT t.
+Proof.
+ intros. eapply prim_types_closed in H; rip.
+Qed.
+Hint Resolve prim_types_closed_result.
+
+
